new/proof/github_com/sanjit_bhat/pav/prelude.v
@@ -5,6 +5,7 @@ or unintended name shadows. *)
 
 (* for inG's. not exported. *)
 From New.proof Require Import proof_prelude.
+From New.proof Require Import sync.
 
 (* add extra dependencies. *)
 From RecordUpdate Require Export RecordSet.
@@ -50,12 +51,11 @@ Class sigpredG Σ := {
 
 Class pavG Σ := {
   #[global] pavG_sigpred :: sigpredG Σ;
-  (* ghost_map uid (gset (ver, pk)). *)
-  #[global] pavG_puts :: ghost_mapG Σ w64 (gset (w64 * list w8));
   (* serverσ.hist. *)
   #[global] pavG_serv_hist :: mono_listG (list w8 * (gmap w64 (list $ list w8))) Σ;
   (* serverσ.pending. each uid has a mono_list of (ver, pk). *)
   #[global] pavG_serv_uids :: mono_listG (w64 * list w8) Σ;
+  #[global] pavG_sync :: syncG Σ;
 }.
 
 (* misc. TODO: these should definitely go into separate file. *)
